src/Set.v
@@ -1,0 +1,20 @@
+
+Class set(T E: Type) := mkSet {
+  empty_set: T;
+  singleton_set: E -> T;
+  union: T -> T -> T;
+  intersect: T -> T -> T;
+  diff: T -> T -> T;
+  contains: T -> E -> Prop;
+}.
+
+Notation "x '\in' s" := (contains s x) (at level 39, no associativity).
+
+Instance Function_Set(E: Type): set (E -> Prop) E := {|
+  empty_set := fun _ => False;
+  singleton_set y := fun x => x = y;
+  union := fun s1 s2 => fun x => s1 x \/ s2 x;
+  intersect := fun s1 s2 => fun x => s1 x /\ s2 x;
+  diff := fun s1 s2 => fun x => s1 x /\ ~ s2 x;
+  contains := fun s => s
+|}.
