src/StateCalculus.v
@@ -27,44 +27,64 @@ Section StateCalculus.
 
   Definition subset(vs1 vs2: vars) := forall x, x \in vs1 -> x \in vs2.
 
-  Hint Unfold extends only_differ undef : unfold_state_calculus.
+  Lemma intersect_spec: forall (x: var) (A B: vars),
+    x \in (intersect A B) <-> x \in A /\ x \in B.
+  Proof. intros. cbv. tauto. Qed.
 
-  Ltac unf := repeat autounfold with unfold_state_calculus.
+  Lemma union_spec: forall (x: var) (A B: vars),
+    x \in (union A B) <-> x \in A \/ x \in B.
+  Proof. intros. cbv. tauto. Qed.
 
-Lemma intersect_spec: forall (x: var) (A B: vars),
-  x \in (intersect A B) <-> x \in A /\ x \in B.
-Proof. intros. cbv. tauto. Qed.
+  Lemma diff_spec: forall (x: var) (A B: vars),
+    x \in (diff A B) <-> x \in A /\ ~ x \in B.
+  Proof. intros. cbv. tauto. Qed.
 
-Lemma union_spec: forall (x: var) (A B: vars),
-  x \in (union A B) <-> x \in A \/ x \in B.
-Proof. intros. cbv. tauto. Qed.
+  Lemma singleton_set_spec: forall (x y: var),
+    x \in singleton_set y <-> x = y.
+  Proof. intros. cbv. tauto. Qed.
 
-Lemma diff_spec: forall (x: var) (A B: vars),
-  x \in (diff A B) <-> x \in A /\ ~ x \in B.
-Proof. intros. cbv. tauto. Qed.
+  Lemma get_put: forall (s: state) (x y: var) (v: val),
+    get (put s x v) y = if dec (x = y) then Some v else get s y.
+  Proof.
+    intros. destruct (dec (x = y)).
+    - subst. rewrite get_put_same. reflexivity.
+    - rewrite get_put_diff by assumption. reflexivity.
+  Qed.
 
-Lemma singleton_set_spec: forall (x y: var),
-  x \in singleton_set y <-> x = y.
-Proof. intros. cbv. tauto. Qed.
+End StateCalculus.
 
-Hint Rewrite intersect_spec union_spec diff_spec singleton_set_spec : rewrite_set_op_specs.
 
-Lemma get_put: forall (s: state) (x y: var) (v: val),
-  get (put s x v) y = if dec (x = y) then Some v else get s y.
-Proof.
-  intros. destruct (dec (x = y)).
-  - subst. rewrite get_put_same. reflexivity.
-  - rewrite get_put_diff by assumption. reflexivity.
-Qed.
+Hint Unfold extends only_differ undef : unfold_state_calculus.
+Ltac unf := repeat autounfold with unfold_state_calculus.
 
-Hint Rewrite get_put : rewrite_state_op_specs.
+Hint Rewrite @intersect_spec @union_spec @diff_spec @singleton_set_spec : rewrite_set_op_specs.
 
-  Ltac state_calc :=
-    unf; intros; autorewrite with rewrite_set_op_specs rewrite_state_op_specs in *;
-    repeat match goal with
-    | x: ?T, H: forall (y: ?T), _ |- _ => unique pose proof (H x)
-    end;
-    repeat (intuition (auto || congruence) || destruct_one_dec_eq).
+(* only needed to get the DecidableEq *)
+Ltac rewrite_get_put :=
+  repeat match goal with
+  | D: DecidableEq ?Var |- context [@get _ ?Var _ _ (put _ _ _) _] =>
+     rewrite (@get_put Var D) in *
+  | D: DecidableEq ?Var, _: context [@get _ ?Var _ _ (put _ _ _) _] |- _ =>
+     rewrite (@get_put Var D) in *
+  end.
+
+Ltac state_calc :=
+  unf; intros; autorewrite with rewrite_set_op_specs in *; rewrite_get_put;
+  repeat match goal with
+  | x: ?T, H: forall (y: ?T), _ |- _ => unique pose proof (H x)
+  end;
+  repeat (intuition (auto || congruence) || destruct_one_dec_eq).
+
+
+Section Tests.
+
+  Context {var: Type}. (* variable name (key) *)
+  Context {dec_eq_var: DecidableEq var}.
+  Context {val: Type}. (* value *)
+  Context {dec_eq_val: DecidableEq val}.
+  Context {state: Type}.
+  Context {stateMap: Map state var val}.
+
 
   Lemma extends_refl: forall s, extends s s.
   Proof. state_calc. Qed.
@@ -140,4 +160,4 @@ Hint Rewrite get_put : rewrite_state_op_specs.
     only_differ s d (put s x v).
   Proof. state_calc. Qed.
 
-End StateCalculus.
+End Tests.
